Source/DafnyRuntime/DafnyRuntimeDafny/src/atomicBox.dfy
@@ -1,0 +1,51 @@
+
+include "array.dfy"
+include "frames.dfy"
+
+module {:options "/functionSyntax:4"} AtomicBoxes {
+  import opened Arrays
+  import opened Frames
+
+  trait {:termination false} AtomicBox<T> extends Validatable {
+
+    ghost predicate Valid()
+      reads this, Repr
+      ensures Valid() ==> Repr == {}
+
+    ghost const inv: T -> bool
+
+    method {:extern} Put(t: T)
+      requires inv(t)
+
+    method {:extern} Get() returns (t: T)
+      ensures inv(t)
+  }
+
+  // Feasibility implementation
+  // DO NOT USE THIS as it is not guaranteed to be atomic!
+  //
+  // Using Array<T> as an arbitrary type that needs an invariant.
+  // class DafnyNotActuallyAtomicBox<T> extends AtomicBox<Array<T>> {
+
+  //   var value: Array<T>
+
+  //   constructor(inv: Array<T> -> bool, value: Array<T>) 
+  //     requires inv(value)
+  //   {
+  //     this.inv := inv;
+  //     this.value := value;
+  //   }
+
+  //   method Put(value: Array<T>)
+  //     requires inv(value)
+  //   {
+  //     this.value := value;
+  //   }
+
+  //   method Get() returns (value: Array<T>)
+  //     ensures inv(value)
+  //   {
+  //     return this.value;
+  //   }
+  // }
+}
